<?xml version="1.0" encoding="UTF-8"?>

<section xml:id="sec-comb" xmlns:xi="http://www.w3.org/2001/XInclude">
  <title>Combinations</title>

  
<p>
  Select the letters <m>A, B, C</m> by taking three at a time.
</p>
<p>
  Here:
  <me>
    ABC
  </me>
  
  so again <m>6</m> permutations.
</p>

<p>
 Find all combinations of letters <m>A, B, C, D</m> by taking three at a time.
</p>

<p>
 <me>
  ABC, ABD, ACD, BCD
 </me>
</p>

<theorem xml:id="thm-comb1">
  <statement>
    <p>
      The number of all combinatios of <m>n</m> distinct objects, taken <m>r</m> at a time, where <m>0\leq r \leq n</m> 
     is given by <m> (C,r) \quad \text{ or, } \quad  ^nC_r</m>. Here, 
      <me>
      ^nC_r = \frac{n!}{r!(n-r)!}.
      </me>
      </p>
  </statement>
</theorem>

<corollary xml:id="cor-comb_1th1">
  <statement>
    <p>
     <me>
      ^nC_r = \frac{n(n-1)(n-2) \ldots \text{ to } r \text{ factors }}{r!} 
     </me>
    </p>
  </statement>
</corollary>


<corollary xml:id="cor-comb_2th1">
  <statement>
    <p>
     <me>
      ^nC_n =  ^nC_0 = 1. 
     </me>
    </p>
  </statement>
</corollary>


<corollary xml:id="cor-comb_3th1">
  <statement>
    <p>
     <me>
      ^nC_r =  \frac{^nP_r}{r!}. 
     </me>
    </p>
  </statement>
</corollary>



<theorem xml:id="thm-comb2">
  <statement>
    <p>
      For <m>0 \leq r \leq n,</m> we have 
      <me>
        ^nC_r = ^nC_{(n-r)}
        </me>
    </p>
    </statement>
</theorem>

<theorem xml:id="thm-comb3">
  <statement>
    <p>
      If <me>
        ^nC_x = ^nC_y 
      </me>
      and <m>x\neq y</m>, then we have 
      <me>x+y =n.</me>
    </p>
  </statement>
</theorem>

<theorem xml:id="thm-comb4">
  <statement>
    <p>
      Let <m>1 \leq r \leq n,</m> then, we have 
      <me>
        ^nC_r + ^nC_{(r-1)} = ^{(n+1)}C_r \quad \text{ Pascal's Rule}
      </me>
          </p>
          <p>
            For example: (i) <me>
              ^{10}C_4 + ^{10}C_3 = ^{11}C_4
            </me>
          </p>
  </statement>
</theorem>


<theorem xml:id="thm-comb5">
  <statement>
    <p>
      If <m>1\leq r \leq n,</m> then we have 
      <me>
        n \times ^{(n-1)}C_{(r-1)} = (n-r+1) \times ^nC_{(r-1)}
      </me>
      
    </p>
  </statement>
</theorem>

<theorem xml:id="thm-comb6">
  <statement>
    <p>
      If <m>n</m> and <m>r</m> are positive integers such that <m>1\leq r\leq n,</m> then we have 
      <ol marker ="I">
        <li>
          <p>
            <me>
              \frac{^nC_{r}}{^nC_{(r-1)}} = \frac{n-r+1}{r}
            </me>
          </p>
        </li>
        <li>
          <p>
            <me>
              \frac{^nC_{r}}{^{(n-1)}C_{(r-1)}} = \frac{n}{r}
            </me> 
          </p>
        </li>
        <li>
          <p>
            <me>
              \frac{^nC_{r}}{^nC_{(r+1)}} = \frac{r+1}{n-r}.
            </me>
          </p>
        </li>
      </ol>
    </p>
  </statement>
</theorem>


</section>